adding falcon spec

crypto_specs/mq_norm.s.dfy
@@ -16,10 +16,20 @@ module mq_norm_s(MQ: ntt_param_s) {
         if e <= Q_HLAF then e else e as int - MQ.Q
     }
 
+    function normalize_elems(s: seq<MQ.elem>): seq<nelem>
+    {
+        seq(|s|, i requires 0 <= i < |s| => normalize(s[i]))
+    }
+
     // -Q/2 <= e < Q/2 -> 0 <= e <= Q 
     function denormalize(e: nelem): MQ.elem
     {
         if e >= 0 then e else e + MQ.Q
+    }
+
+    function denormalize_nelems(s: seq<nelem>): seq<MQ.elem>
+    {
+        seq(|s|, i requires 0 <= i < |s| => denormalize(s[i]))
     }
 
     lemma normalize_inverse(e: MQ.elem)
@@ -29,7 +39,23 @@ module mq_norm_s(MQ: ntt_param_s) {
     lemma denormalize_inverse(e: nelem)
         ensures normalize(denormalize(e)) == e;
     {
-        MQ.Nth_root_lemma();
+    }
+
+    lemma square_positive_lemma(a: int)
+        ensures a * a >= 0;
+
+    function l2norm_squared(s1: seq<nelem>, s2: seq<nelem>, i: nat): nat
+        requires |s1| == |s2|
+        requires i <= |s1|
+    {
+        if i == 0 then
+            0
+        else
+            var v1, v2 := s1[i-1] as int, s2[i-1] as int;
+            square_positive_lemma(v1);
+            square_positive_lemma(v2);
+            var vv1, vv2 := v1 * v1, v2 * v2;
+            l2norm_squared(s1, s2, i-1) + vv1 + vv2
     }
 }
 
