crypto_specs/falcon.s.dfy
@@ -1,0 +1,34 @@
+include "mq_poly.s.dfy"
+include "mq_norm.s.dfy"
+
+abstract module falcon_s(CMQ: ntt_param_s) {
+    import MQP = mq_poly_s(CMQ)
+    import MQN = mq_norm_s(CMQ)
+
+	type elem = CMQ.elem
+    type nelem = MQN.nelem
+	type n_elems = CMQ.n_elems
+
+	// const Q := CMQ.Q;
+	const N := CMQ.N; 
+
+    function bound(): nat
+
+    predicate falcon_verify(c0: seq<elem>, s2: seq<nelem>, h: seq<elem>)
+        requires |c0| == |s2| == |h| == N.full;
+    {
+        var tt0 := MQN.denormalize_nelems(s2);
+        var tt1 := MQP.poly_mod(MQP.poly_mul(tt0, h), MQP.n_ideal());
+        var tt2 := MQP.poly_sub(tt1, c0);
+        var s1 := MQN.normalize_elems(tt2);
+        MQN.l2norm_squared(s1, s2, N.full) < bound()
+    }
+}
+
+
+module falcon_512_i refines falcon_s(ntt512_param_i)
+{
+    function bound(): nat {
+        0x29845d6
+    }
+}
